started coq npc reduction, refactoring pcc

coq/pcc/program_model.v
@@ -1,507 +1,482 @@
-
 Require Export expressions_assertions.
 Require Export Bool.
 Require Import list_utils.
 Require Import ssreflect.
 
-Section program_model.
+Section ProgramModel.
   
-  Open Scope type_scope.
-  
-  Definition ghost_update := ghostid * expr.
-  
-  Inductive instr : Set :=
-  | aload (_: nat)
-  | astore (_: nat)
-  | athrow
-  | dup
-  | getfield (_: fieldid)
-  | getstatic (_: classid) (_: fieldid)
-  | goto (_: label)
-  | iadd
-  | iconst (_: Z)
-  | ifeq (_: label)
-  | invoke (_: classid) (_: methid)
-  | putstatic (_: classid) (_: fieldid)
-  | ldc (_: jvalue)
-  | exit
-  | ret
-  | nop
-  | ghost_instr (_: ghost_update).
-  
-  
-  (* Exception handler records (Rows in the exception handler table) *)
-  Record eh_record : Set := {
-    start_label  : label;
-    end_label    : label;
-    target_label : label;
-    handled_classes : classid
-  }.
-  Definition eh_table := list eh_record.
-  
-  
-  (* A label function is used to look up successor-labels.
-     It used to be 'S' (the nat successor-funciotn) but that quickly became
-     insufficient when inserting ghost-instructions.
-  *)
-  Definition label_function := label -> label.
-  
-  
-  (* We're skipping the regular method definition and jump straight to the
-     extended version which includes assertions. *)
-  Record method := {
-    code_of: label -> instr;
-    annotations_of : label -> ast;
-    eh_table_of: eh_table;
-    label_function_of: label_function
-  }.
-  
-  
-  (* No field declarations at this point. Wi simply assume that all fields accessed
-     by the program has been properly declared. *)
-  Definition class := methid -> method.
-  
-  
-  (* Local variables store. *)
-  Definition lstore := nat -> jvalue.
-  Definition emptylstore : lstore := fun x => undefval.
-  Definition upd (ls:lstore) (n:nat) (v:jvalue) : lstore :=
-    fun x => if beq_nat x n then v else ls x.
-  
-  
-  (* A heap consists of a dynamic part (dheap) and static part (sheap). *)
-  Definition dheap := loc -> option object.
-  Definition sheap := classid -> fieldid -> option jvalue.
-  Definition heap := dheap * sheap.
-  
-  Definition empty_heap : heap := (fun l => None, fun c f => None).
-  Definition upd_sheap (h:heap) (cid:classid) (fid:fieldid) (v:jvalue) : heap :=
-    (fst h, fun c f => if beq_nat c cid && beq_nat f fid then Some v else (snd h) c f).
-  
-  Notation "ls '[[' n '⟼' v ']]'" := (upd ls n v) (at level 90).
-  
-  
-  (* Activation records. *)
-  Inductive act_record : Set :=
-  | normal (_: classid) (_: methid) (_: label) (_: stack) (_: lstore)
-  | exceptional (_: loc).
-  
-  
-  Record program := {
-    classes: classid -> class;
-    inv: ast
-  }.
-  
-  (* Main class and main method are assumed to be these constants. *)
-  Definition maincid : classid := O.
-  Definition mainmid : methid := O.
-  
-  
-  Definition ghost_valuation := ghostid -> value.
-  (* We assume that the default value for ghost variables is 0. (Since the undefval is
-     reserved for the notion of "going wrong".) *)
-  Definition initial_gv : ghost_valuation := fun l => intval 0. 
-  Definition upd_gv (gv: ghost_valuation) (var: ghostid) (val: value) : ghost_valuation :=
-    (fun v => if beq_nat v var then val else gv v).
-  
-  
-  (* We go straight to extended configurations. *)
-  Definition conf := ghost_valuation * heap * (list act_record).
-  Definition execution := list conf.
-  
-  
-  
-  (* Convenience access methods  *)
-  Definition instr_at (p: program) c m l : instr := code_of (classes p c m) l.
-  Definition minstr_at (m: method) l : instr := code_of m l.
-  Definition ast_at   (p: program) c m l : ast   := annotations_of (classes p c m) l.
-  Definition successor (p: program) c m l := label_function_of (classes p c m) l.
-  Definition stack_of (c: conf) : option stack :=
-    match c with (_, _, (normal _ _ _ s _)::_) => Some s | _ => None end.
-  Definition lstore_of (c: conf) : option lstore :=
-    match c with (_, _, (normal _ _ _ _ ls)::_) => Some ls | _ => None end.
-  Definition class_of (c: conf) : option classid :=
-    match c with (_, _, (normal c _ _ _ _)::_) => Some c | _ => None end.
-  Definition meth_of (c: conf) : option methid :=
-    match c with (_, _, (normal _ m _ _ _)::_) => Some m | _ => None end.
-  Definition heap_of (c: conf) : heap := snd (fst c).
-  Definition ars_of (c: conf) : (list act_record) := snd c.
-  Definition ghost_valuation_of (c: conf) : ghost_valuation := fst (fst c).
-  Definition current_instr (p: program) (cnf: conf) : option instr :=
-    match cnf with (_, _, (normal c m pc _ _)::_) => Some (instr_at p c m pc) | _ => None end.
-  Definition current_ast (p: program) (cnf: conf) : option ast :=
-    match cnf with (_, _, (normal c m pc _ _)::_) => Some (ast_at p c m pc) | _ => None end.
-  Definition current_label (cnf: conf) : option label :=
-    match cnf with (_, _, (normal _ _ pc _ _)::_) => Some pc | _ => None end.
-  
-  Lemma current_to_instr_at :
-    forall pg p c m pc s l1 l i, current_instr pg (p, normal c m pc s l1 :: l) = Some i ->
-      instr_at pg c m pc = i.
-  Proof.
-    intros.
-    inversion H.
-    destruct p.
-    inversion H1; subst.
-    reflexivity.
-  Qed.
+Open Scope type_scope.
 
-  Lemma instr_at_to_current :
-    forall pg p c m pc s l1 l i, instr_at pg c m pc = i -> current_instr pg (p, normal c m pc s l1 :: l) = Some i.
-  Proof.
-    intros.
-    unfold current_instr.
-    destruct p.
-    rewrite H.
-    reflexivity.
-  Qed.
+Definition ghost_update := ghostid * expr.
 
+Inductive instr : Set :=
+| aload (_: nat)
+| astore (_: nat)
+| athrow
+| dup
+| getfield (_: fieldid)
+| getstatic (_: classid) (_: fieldid)
+| goto (_: label)
+| iadd
+| iconst (_: Z)
+| ifeq (_: label)
+| invoke (_: classid) (_: methid)
+| putstatic (_: classid) (_: fieldid)
+| ldc (_: jvalue)
+| exit
+| ret
+| nop
+| ghost_instr (_: ghost_update).
+
+(* Exception handler records (rows in the exception handler table) *)
+Record eh_record : Set := {
+  start_label  : label;
+  end_label    : label;
+  target_label : label;
+  handled_classes : classid
+}.
+
+Definition eh_table := list eh_record.
+
+(* 
+   A label function is used to look up successor-labels. It used to 
+   be 'S' (the nat successor-funciotn) but that quickly became insufficient 
+   when inserting ghost-instructions.
+*)
+Definition label_function := label -> label.
+
+
+(* 
+   We're skipping the regular method definition and jump straight to the
+   extended version which includes assertions. 
+*)
+Record method := {
+  code_of: label -> instr;
+  annotations_of : label -> ast;
+  eh_table_of: eh_table;
+  label_function_of: label_function
+}.
+
+(* 
+   No field declarations at this point. Wi simply assume that all fields 
+   accessed by the program has been properly declared. 
+ *)
+Definition class := methid -> method.
+
+(* Local variables store. *)
+Definition lstore := nat -> jvalue.
+
+Definition emptylstore : lstore := fun x => undefval.
+
+Definition upd (ls:lstore) (n:nat) (v:jvalue) : lstore :=
+  fun x => if beq_nat x n then v else ls x.
+
+(* A heap consists of a dynamic part (dheap) and static part (sheap). *)
+Definition dheap := loc -> option object.
+
+Definition sheap := classid -> fieldid -> option jvalue.
+
+Definition heap := dheap * sheap.
+
+Definition empty_heap : heap := (fun l => None, fun c f => None).
+
+Definition upd_sheap (h:heap) (cid:classid) (fid:fieldid) (v:jvalue) : heap :=
+  (fst h, fun c f => if beq_nat c cid && beq_nat f fid then Some v else (snd h) c f).
+
+Notation "ls '[[' n '⟼' v ']]'" := (upd ls n v) (at level 90).
+
+(* Activation records. *)
+Inductive act_record : Set :=
+| normal (_: classid) (_: methid) (_: label) (_: stack) (_: lstore)
+| exceptional (_: loc).
+
+Record program := {
+  classes: classid -> class;
+  inv: ast
+}.
+
+(* Main class and main method are assumed to be these constants. *)
+Definition maincid : classid := O.
+
+Definition mainmid : methid := O.
+
+Definition ghost_valuation := ghostid -> value.
+
+(* We assume that the default value for ghost variables is 0. (Since the undefval is
+   reserved for the notion of "going wrong".) *)
+Definition initial_gv : ghost_valuation := fun l => intval 0. 
+
+Definition upd_gv (gv: ghost_valuation) (var: ghostid) (val: value) : ghost_valuation :=
+  (fun v => if beq_nat v var then val else gv v).
+
+(* We go straight to extended configurations. *)
+Definition conf := ghost_valuation * heap * (list act_record).
+
+Definition execution := list conf.
+
+(* Convenience access methods  *)
+Definition instr_at (p: program) c m l : instr := code_of (classes p c m) l.
+
+Definition minstr_at (m: method) l : instr := code_of m l.
+
+Definition ast_at   (p: program) c m l : ast   := annotations_of (classes p c m) l.
+
+Definition successor (p: program) c m l := label_function_of (classes p c m) l.
+
+Definition stack_of (c: conf) : option stack :=
+  match c with (_, _, (normal _ _ _ s _)::_) => Some s | _ => None end.
+
+Definition lstore_of (c: conf) : option lstore :=
+  match c with (_, _, (normal _ _ _ _ ls)::_) => Some ls | _ => None end.
+
+Definition class_of (c: conf) : option classid :=
+  match c with (_, _, (normal c _ _ _ _)::_) => Some c | _ => None end.
+
+Definition meth_of (c: conf) : option methid :=
+  match c with (_, _, (normal _ m _ _ _)::_) => Some m | _ => None end.
+
+Definition heap_of (c: conf) : heap := snd (fst c).
+
+Definition ars_of (c: conf) : (list act_record) := snd c.
+
+Definition ghost_valuation_of (c: conf) : ghost_valuation := fst (fst c).
+
+Definition current_instr (p: program) (cnf: conf) : option instr :=
+  match cnf with (_, _, (normal c m pc _ _)::_) => 
+    Some (instr_at p c m pc) | _ => None end.
+
+Definition current_ast (p: program) (cnf: conf) : option ast :=
+  match cnf with (_, _, (normal c m pc _ _)::_) => 
+    Some (ast_at p c m pc) | _ => None end.
+
+Definition current_label (cnf: conf) : option label :=
+  match cnf with (_, _, (normal _ _ pc _ _)::_) => Some pc | _ => None end.
+
+Lemma current_to_instr_at : forall pg p c m pc s l1 l i, 
+  current_instr pg (p, normal c m pc s l1 :: l) = Some i ->
+  instr_at pg c m pc = i.
+Proof.
+move => pg p c m pc s l1 l i H.
+inversion H as [H0].
+move: p H H0; case => g h H H0.
+by inversion H0.
+Qed.
+
+Lemma instr_at_to_current : forall pg p c m pc s l1 l i, 
+  instr_at pg c m pc = i -> current_instr pg (p, normal c m pc s l1 :: l) = Some i.
+Proof.
+move => pg p c m pc s l1 l i H.
+rewrite /current_instr.
+case: p => g h.
+by rewrite H.
+Qed.
 
 (*
-To  show ∥wp(A)∥ C <-> ∥A∥ C' later on, we need a lemma (in the neg case) relating aeval and aeval_f in the following way:
+  To  show ∥wp(A)∥ C <-> ∥A∥ C' later on, we need a lemma (in the neg case) 
+  relating aeval and aeval_f in the following way:
 
-(aeval a c <-> aeval a' c') -> (aeval_f a c <-> aeval_f a' c')       (1)
+  (aeval a c <-> aeval a' c') -> (aeval_f a c <-> aeval_f a' c')       (1)
 
-This fact requires more than just [aeval a c -> ~aeval_f a c] and vice versa,
-since if there is an undefined expression (s.t. [~aeval undef c] and [~aeval_f undef c]) we get the following counter example:
+  This fact requires more than just [aeval a c -> ~aeval_f a c] and vice versa,
+  since if there is an undefined expression (s.t. [~aeval undef c] and 
+  [~ aeval_f undef c]) we get the following counter example:
 
-(aeval ff c <-> aeval undef c') -> (aeval_f ff c <-> aeval_f undef c')
+  (aeval ff c <-> aeval undef c') -> (aeval_f ff c <-> aeval_f undef c')
 
-Fact (1) relies on a stronger fact that
+  Fact (1) relies on a stronger fact that
 
-~(aeval a c <-> aeval_f a c)      (2)
+  ~ (aeval a c <-> aeval_f a c)      (2)
 
-Showing (2) requires that aeval_f is true/defined for all cases in which aeval is not true/defined.
-for example, if the heap is ill-typed, this has to be taken into account in aeval_f.
+  Showing (2) requires that aeval_f is true/defined for all cases in which
+  aeval is not true/defined. For example, if the heap is ill-typed, this has 
+  to be taken into account in aeval_f.
 
-This in turn requires that all expressions can be evaluated to a value, no matter the context.
+  This in turn requires that all expressions can be evaluated to a value, no
+  matter the context.
 *)
 
 Definition is_intval (v: value) : Prop := exists i, v = intval i.
 
 Inductive eeval : expr -> conf -> value -> Prop :=
-  | e_val          : forall c v, eeval (valexp v) c v
-  | e_nsfield      : forall gv c e dh sh ars f l obj, c = (gv, (dh, sh), ars) -> eeval e c (refval l) -> dh l = Some obj -> eeval (nsfield e f) c (obj f)
-  | e_sfield       : forall gv c dh sh ars cid f v, c = (gv, (dh, sh), ars) -> sh cid f = Some v -> eeval (sfield cid f) c v
-  | e_ghosterr        : forall c, eeval ghost_errval c ghost_errval
-  | e_plus         : forall c e1 e2 i j, eeval e1 c (intval i) -> eeval e2 c (intval j) -> eeval (plus e1 e2) c (intval (i + j))
-  | e_guard_true   : forall c eg et ef v, eeval eg c (boolval true ) -> eeval et c v -> eeval (guarded eg et ef) c v
-  | e_guard_other  : forall c eg et ef v, eeval eg c (boolval false) -> eeval ef c v -> eeval (guarded eg et ef) c v
-  | e_stack        : forall c n s, stack_of c = Some s -> eeval (stackexp n) c (s[[n]])
-  | e_local        : forall c n ls, lstore_of c = Some ls -> eeval (local n) c (ls n)
-  | e_ghostvar     : forall c gvarid, eeval (ghost_var gvarid) c ((ghost_valuation_of c) gvarid)
-  | e_nsfield_err1 : forall c e v f, eeval e c v -> (forall l, v <> refval l) -> eeval (nsfield e f) c undefval
-  | e_nsfield_err2 : forall gv c e dh sh ars f l, c = (gv, (dh, sh), ars) -> eeval e c (refval l) -> dh l = None -> eeval (nsfield e f) c undefval
-  | e_sfield_err   : forall gv c dh sh ars cid f, c = (gv, (dh, sh), ars) -> sh cid f = None -> eeval (sfield cid f) c undefval
-  | e_plus_err     : forall c e1 e2 v1 v2, eeval e1 c v1 -> eeval e2 c v2 -> ~is_intval v1 \/ ~is_intval v2 -> eeval (plus e1 e2) c undefval
-  | e_guard_err    : forall c eg et ef v, eeval eg c v -> (forall b, v <> boolval b) -> eeval (guarded eg et ef) c undefval.
+| e_val : forall c v, eeval (valexp v) c v
+| e_nsfield : forall gv c e dh sh ars f l obj, c = (gv, (dh, sh), ars) -> 
+    eeval e c (refval l) -> dh l = Some obj -> eeval (nsfield e f) c (obj f)
+| e_sfield : forall gv c dh sh ars cid f v, c = (gv, (dh, sh), ars) -> 
+    sh cid f = Some v -> eeval (sfield cid f) c v
+| e_ghosterr : forall c, eeval ghost_errval c ghost_errval
+| e_plus : forall c e1 e2 i j, eeval e1 c (intval i) -> 
+    eeval e2 c (intval j) -> eeval (plus e1 e2) c (intval (i + j))
+| e_guard_true : forall c eg et ef v, eeval eg c (boolval true ) -> 
+    eeval et c v -> eeval (guarded eg et ef) c v
+| e_guard_other : forall c eg et ef v, eeval eg c (boolval false) -> 
+    eeval ef c v -> eeval (guarded eg et ef) c v
+| e_stack : forall c n s, stack_of c = Some s -> eeval (stackexp n) c (s[[n]])
+| e_local : forall c n ls, lstore_of c = Some ls -> eeval (local n) c (ls n)
+| e_ghostvar : forall c gvarid, eeval (ghost_var gvarid) c ((ghost_valuation_of c) gvarid)
+| e_nsfield_err1 : forall c e v f, eeval e c v -> (forall l, v <> refval l) -> 
+    eeval (nsfield e f) c undefval
+| e_nsfield_err2 : forall gv c e dh sh ars f l, c = (gv, (dh, sh), ars) -> 
+    eeval e c (refval l) -> dh l = None -> eeval (nsfield e f) c undefval
+| e_sfield_err : forall gv c dh sh ars cid f, c = (gv, (dh, sh), ars) -> 
+    sh cid f = None -> eeval (sfield cid f) c undefval
+| e_plus_err : forall c e1 e2 v1 v2, eeval e1 c v1 -> eeval e2 c v2 -> 
+    ~ is_intval v1 \/ ~ is_intval v2 -> eeval (plus e1 e2) c undefval
+| e_guard_err : forall c eg et ef v, eeval eg c v -> (forall b, v <> boolval b) -> 
+    eeval (guarded eg et ef) c undefval.
 
-
-
-
-
+(* Transitions (activation record related) *)
+Inductive artrans : program -> act_record -> act_record -> Prop :=
+| tr_aload : forall p c m pc n s ls ar1 ar2,
+    instr_at p c m pc = aload n ->
+    ar1 = normal c m pc s ls ->
+    ar2 = normal c m (successor p c m pc) (ls n::s) ls ->
+    artrans p ar1 ar2
+| tr_astore : forall p c m pc s n ls v ar1 ar2,
+    instr_at p c m pc = astore n ->
+    ar1 = normal c m pc (v::s) ls ->
+    ar2 = normal c m (successor p c m pc) s (ls[[n ⟼ v]]) ->
+    artrans p ar1 ar2
+| tr_dup : forall p c m pc s ls v ar1 ar2,
+    instr_at p c m pc = dup ->
+    ar1 = normal c m pc (v::s) ls ->
+    ar2 = normal c m (successor p c m pc) (v::v::s) ls ->
+    artrans p ar1 ar2
+| tr_goto : forall p c m l pc s ls ar1 ar2,
+    instr_at p c m pc = goto l ->
+    ar1 = normal c m pc s ls ->
+    ar2 = normal c m l  s ls ->
+    artrans p ar1 ar2
+| tr_iconst : forall p c m pc n ls s ar1 ar2,
+    instr_at p c m pc = iconst n ->
+    ar1 = normal c m pc s ls ->
+    ar2 = normal c m (successor p c m pc) ((intval n)::s) ls ->
+    artrans p ar1 ar2
+| tr_ldc : forall p c m pc s ls v ar1 ar2,
+    instr_at p c m pc = ldc v ->
+    ar1 = normal c m pc s ls ->
+    ar2 = normal c m (successor p c m pc) (v::s) ls ->
+    artrans p ar1 ar2
+| tr_ifeq_true : forall p c m pc s ls l v ar1 ar2,
+    instr_at p c m pc = ifeq l ->
+    v = boolval true ->
+    ar1 = normal c m pc (v::s) ls ->
+    ar2 = normal c m l s ls ->
+    artrans p ar1 ar2
+| tr_ifeq_false : forall p c m pc s ls l v ar1 ar2,
+    instr_at p c m pc = ifeq l ->
+    v = boolval false ->
+    ar1 = normal c m pc (v::s) ls ->
+    ar2 = normal c m l s ls ->
+    artrans p ar1 ar2.
+    
+(* Transitions (heap releated) *)
+Inductive htrans : program -> conf -> conf -> Prop :=
+| tr_putstatic : forall p c cid fid ars m pc v s ls h c1 c2 ar1 ar2 gv,
+    instr_at p c m pc = putstatic cid fid ->
+    ar1 = normal c m pc (v::s) ls ->
+    ar2 = normal c m (successor p c m pc) (v::s) ls ->
+    c1 = (gv, h, ar1::ars) ->
+    c2 = (gv, upd_sheap h cid fid v, ar2::ars) ->
+    htrans p c1 c2
+| tr_getstatic : forall p c cid fid ars m pc v s ls h c1 c2 ar1 ar2 gv,
+    instr_at p c m pc = getstatic cid fid ->
+    ar1 = normal c m pc s ls ->
+    ar2 = normal c m (successor p c m pc) (v::s) ls ->
+    c1 = (gv, h, ar1::ars) ->
+    c2 = (gv, h, ar2::ars) ->
+    htrans p c1 c2.
   
-  (* Transitions (activation record related) *)
-  Inductive artrans : program -> act_record -> act_record -> Prop :=
-  | tr_aload : forall p c m pc n s ls ar1 ar2,
-      instr_at p c m pc = aload n ->
-      ar1 = normal c m pc s ls ->
-      ar2 = normal c m (successor p c m pc) (ls n::s) ls ->
-      artrans p ar1 ar2
-  | tr_astore : forall p c m pc s n ls v ar1 ar2,
-      instr_at p c m pc = astore n ->
-      ar1 = normal c m pc (v::s) ls ->
-      ar2 = normal c m (successor p c m pc) s (ls[[n ⟼ v]]) ->
-      artrans p ar1 ar2
-  | tr_dup : forall p c m pc s ls v ar1 ar2,
-      instr_at p c m pc = dup ->
-      ar1 = normal c m pc (v::s) ls ->
-      ar2 = normal c m (successor p c m pc) (v::v::s) ls ->
-      artrans p ar1 ar2
-  | tr_goto : forall p c m l pc s ls ar1 ar2,
-      instr_at p c m pc = goto l ->
-      ar1 = normal c m pc s ls ->
-      ar2 = normal c m l  s ls ->
-      artrans p ar1 ar2
-  | tr_iconst : forall p c m pc n ls s ar1 ar2,
-      instr_at p c m pc = iconst n ->
-      ar1 = normal c m pc s ls ->
-      ar2 = normal c m (successor p c m pc) ((intval n)::s) ls ->
-      artrans p ar1 ar2
-  | tr_ldc : forall p c m pc s ls v ar1 ar2,
-      instr_at p c m pc = ldc v ->
-      ar1 = normal c m pc s ls ->
-      ar2 = normal c m (successor p c m pc) (v::s) ls ->
-      artrans p ar1 ar2
-  | tr_ifeq_true : forall p c m pc s ls l v ar1 ar2,
-      instr_at p c m pc = ifeq l ->
-      v = boolval true ->
-      ar1 = normal c m pc (v::s) ls ->
-      ar2 = normal c m l s ls ->
-      artrans p ar1 ar2
-  | tr_ifeq_false : forall p c m pc s ls l v ar1 ar2,
-      instr_at p c m pc = ifeq l ->
-      v = boolval false ->
-      ar1 = normal c m pc (v::s) ls ->
-      ar2 = normal c m l s ls ->
-      artrans p ar1 ar2.
+(* Ghost instruction transitions *)
+(* Just a stub as of now. *)
+Inductive g_eeval : expr -> ghost_valuation -> value -> Prop :=
+| ge_val : forall s v, g_eeval (valexp v) s v
+| ge_gv : forall gv gid, g_eeval (ghost_var gid) gv (gv gid)
+| ge_nsfield : forall e f gv, g_eeval (nsfield e f) gv undefval
+| ge_sfield : forall gv cid f, g_eeval (sfield cid f) gv undefval
+| ge_stackexp : forall gv n, g_eeval (stackexp n) gv undefval
+| ge_local : forall gv l, g_eeval (local l) gv undefval
+| ge_plus : forall gv e1 e2, g_eeval (plus e1 e2) gv undefval
+| ge_guarded : forall gv e1 e2 e3, g_eeval (guarded e1 e2 e3) gv undefval.
+    
+Inductive ghosttrans : program -> conf -> conf -> Prop :=
+| tr_ghost_upd :
+  forall h ars s ls
+    `(instr_at p c m pc = ghost_instr (gvar, e))
+    `(g_eeval e gv v),
+    ghosttrans p (gv, h, (normal c m pc s ls) :: ars)
+      (upd_gv gv gvar v, h, (normal c m (successor p c m pc) s ls) :: ars).
+    
+(* Transitions (invoke-related) *)
+Inductive invtrans : program -> conf -> conf -> Prop :=
+| tr_invoke : forall p c m pc cid mid s ls c1 c2 h ar1 ar2 ars gv,
+    instr_at p c m pc = invoke cid mid ->
+    ar1 = normal c m pc s ls ->
+    ar2 = normal c m (successor p c m pc) s ls ->
+    c1 = (gv, h, ar1::ars) ->
+    c2 = (gv, h, (normal cid mid O emptystack emptylstore)::ar2::ars) ->
+    invtrans p c1 c2.
+    
+(* Transitions (exceptional) *)
+(* Not implemented as of now. *)  
   
+(* Transitions Combined (Only activation record related as of now.) *)
+Inductive trans : program -> conf -> conf -> Prop :=
+| tr_ar : forall prog ar1 ar2 ars h c1 c2 gv,
+    c1 = (gv, h, ar1::ars) ->
+    c2 = (gv, h, ar2::ars) ->
+    artrans prog ar1 ar2 ->
+    trans prog c1 c2
+| tr_ghost : forall p c c', ghosttrans p c c' -> trans p c c'.
   
-  (* Transitions (heap releated) *)
-  Inductive htrans : program -> conf -> conf -> Prop :=
-  | tr_putstatic : forall p c cid fid ars m pc v s ls h c1 c2 ar1 ar2 gv,
-      instr_at p c m pc = putstatic cid fid ->
-      ar1 = normal c m pc (v::s) ls ->
-      ar2 = normal c m (successor p c m pc) (v::s) ls ->
-      c1 = (gv, h, ar1::ars) ->
-      c2 = (gv, upd_sheap h cid fid v, ar2::ars) ->
-      htrans p c1 c2
-  | tr_getstatic : forall p c cid fid ars m pc v s ls h c1 c2 ar1 ar2 gv,
-      instr_at p c m pc = getstatic cid fid ->
-      ar1 = normal c m pc s ls ->
-      ar2 = normal c m (successor p c m pc) (v::s) ls ->
-      c1 = (gv, h, ar1::ars) ->
-      c2 = (gv, h, ar2::ars) ->
-      htrans p c1 c2.
+Inductive trans_star : program -> execution -> Prop :=
+| tr_star_nil : forall p, trans_star p nil
+| tr_star_sing : forall p c, trans_star p (c :: nil)
+| tr_star_step : forall p c c' e, trans p c c' ->
+    trans_star p (c' :: e) ->
+    trans_star p (c :: c' :: e).
   
-
-  (* Ghost instruction transitions *)
-  (* Just a stub as of now. *)
-  Inductive g_eeval : expr -> ghost_valuation -> value -> Prop :=
-  | ge_val : forall s v, g_eeval (valexp v) s v
-  | ge_gv : forall gv gid, g_eeval (ghost_var gid) gv (gv gid)
-  | ge_nsfield : forall e f gv, g_eeval (nsfield e f) gv undefval
-  | ge_sfield : forall gv cid f, g_eeval (sfield cid f) gv undefval
-  | ge_stackexp : forall gv n, g_eeval (stackexp n) gv undefval
-  | ge_local : forall gv l, g_eeval (local l) gv undefval
-  | ge_plus : forall gv e1 e2, g_eeval (plus e1 e2) gv undefval
-  | ge_guarded : forall gv e1 e2 e3, g_eeval (guarded e1 e2 e3) gv undefval.
-  
-  
-  
-  Inductive ghosttrans : program -> conf -> conf -> Prop :=
-    | tr_ghost_upd :
-      forall h ars s ls
-        `(instr_at p c m pc = ghost_instr (gvar, e))
-        `(g_eeval e gv v),
-        ghosttrans p (gv, h, (normal c m pc s ls) :: ars)
-          (upd_gv gv gvar v, h, (normal c m (successor p c m pc) s ls) :: ars).
-  
-  
-  (* Transitions (invoke-related) *)
-  Inductive invtrans : program -> conf -> conf -> Prop :=
-  | tr_invoke : forall p c m pc cid mid s ls c1 c2 h ar1 ar2 ars gv,
-      instr_at p c m pc = invoke cid mid ->
-      ar1 = normal c m pc s ls ->
-      ar2 = normal c m (successor p c m pc) s ls ->
-      c1 = (gv, h, ar1::ars) ->
-      c2 = (gv, h, (normal cid mid O emptystack emptylstore)::ar2::ars) ->
-      invtrans p c1 c2.
-  
-  
-  (* Transitions (exceptional) *)
-  (* Not implemented as of now. *)
-  
-  
-  (* Transitions Combined (Only activation record related as of now.) *)
-  Inductive trans : program -> conf -> conf -> Prop :=
-  | tr_ar : forall prog ar1 ar2 ars h c1 c2 gv,
-      c1 = (gv, h, ar1::ars) ->
-      c2 = (gv, h, ar2::ars) ->
-      artrans prog ar1 ar2 ->
-      trans prog c1 c2
-  | tr_ghost : forall p c c', ghosttrans p c c' -> trans p c c'.
-  
-
-  Inductive trans_star : program -> execution -> Prop :=
-  | tr_star_nil : forall p, trans_star p nil
-  | tr_star_sing : forall p c, trans_star p (c :: nil)
-  | tr_star_step : forall p c c' e, trans p c c' ->
-                                    trans_star p (c' :: e) ->
-                                    trans_star p (c :: c' :: e).
-  
-
-  Lemma trans_star_seq : forall p c `(trans_star p (e1 ++ c :: nil)) `(trans_star p (c :: e2)),
-    trans_star p (e1 ++ c :: e2).
-  Proof.
-intros.
-induction e1.
-assumption.
-rewrite <- app_comm_cons.
-induction e1.
-simpl.
-apply tr_star_step.
-simpl in trans_star0.
-inversion trans_star0.
-assumption.
-assumption.
-simpl in * |- *.
-apply tr_star_step.
-inversion trans_star0.
-assumption.
-apply IHe1.
-inversion trans_star0.
-assumption.
+Lemma trans_star_seq : forall p c `(trans_star p (e1 ++ c :: nil)) `(trans_star p (c :: e2)),
+  trans_star p (e1 ++ c :: e2).
+Proof.
+move => p c.
+elim => [|c']; first by [].
+case => [|c0 l] IH H0 e2 H1; rewrite -app_comm_cons /=.
+- by apply tr_star_step; first by inversion H0.
+- apply tr_star_step; first by inversion H0.
+  rewrite /= in IH; apply IH; last by [].
+  by inversion H0.
 Qed.
-
 
 Lemma trans_star_suff : forall p e e', trans_star p (e ++ e') -> trans_star p e'.
-intros.
-induction e.
-assumption.
-apply IHe.
-simpl in H.
-inversion H.
-apply tr_star_nil.
-assumption.
+Proof.
+move => p.
+elim => [|c e IH e' H]; first by [].
+by apply IH; inversion H; first by apply tr_star_nil.
 Qed.
 
+Definition initial_conf (c: conf) : Prop := 
+  c = (initial_gv, empty_heap, 
+    (normal maincid mainmid O emptystack (fun n => undefval))::nil).
 
+Inductive execution_of p : execution -> Prop :=
+| exec_intros : forall exec,
+    (forall c, head exec = Some c -> initial_conf c) ->
+    (forall pref c c' suff, exec = pref ++ c :: c' :: suff -> trans p c c') ->
+    execution_of p exec.
 
+(* 
+   An alternative approach would have been to define execution as a dependent
+   inductive type directly based on initial_conf and trans. Such approach,
+   would be cleaner in many ways, but would unfortunately prevent us from
+   using all the nice list lemmas and induction principles in the coq
+   library.
+   
+   Same goes for the approach { ex : list conf | execution_of p ex } since
+   elements of this type are not lists either. 
+*)
 
+Definition max_execution_of p e : Prop :=
+  execution_of p e /\ ~ exists c, execution_of p (e ++ c :: nil).
 
+Lemma exec_nil : forall p, execution_of p nil.
+Proof.
+move => p.
+apply exec_intros; first by [].
+move => pref c c' suffx H.
+by contradict H; auto with datatypes.
+Qed.
 
-  Definition initial_conf (c: conf) : Prop :=
-    c = (initial_gv, empty_heap, (normal maincid mainmid O emptystack (fun n => undefval))::nil).
-  
-  
-  Inductive execution_of p : execution -> Prop :=
-  | exec_intros : forall exec,
-                      (forall c, head exec = Some c -> initial_conf c) ->
-                      (forall pref c c' suff, exec = pref ++ c :: c' :: suff -> trans p c c') ->
-                      execution_of p exec.
-
-  (* An alternative approach would have been to define execution as a dependent
-     inductive type directly based on initial_conf and trans. Such approach,
-     would be cleaner in many ways, but would unfortunately prevent us from
-     using all the nice list lemmas and induction principles in the coq
-     library.
-     
-     Same goes for the approach { ex : list conf | execution_of p ex } since
-     elements of this type are not lists either. *)
-
-  Definition max_execution_of p e : Prop :=
-    execution_of p e /\ ~ exists c, execution_of p (e ++ c :: nil).
-
-  Lemma exec_nil : forall p, execution_of p nil.
-    intros.
-    apply exec_intros.
-    intros.
-    inversion H.
-    intros.
-    contradict H.
-    auto with datatypes.
-  Qed.
-  
-
-  Lemma exec_sing_impl_initial : forall `(execution_of p (c :: nil)), initial_conf c.
-  Proof.
-    move => p c H_exec.
-    inversion H_exec as [exec H_init H_trans H_eq].
-    by apply H_init.
-  Qed.
-
+Lemma exec_sing_impl_initial : forall `(execution_of p (c :: nil)), initial_conf c.
+Proof.
+move => p c H_exec.
+inversion H_exec as [exec H_init H_trans H_eq].
+by apply H_init.
+Qed.
 
 Lemma exec_append : forall `(execution_of p (e ++ c :: nil)) `(trans p c c'),
   execution_of p (e ++ c :: c' :: nil).
-intros.
-inversion execution_of0.
+Proof.
+move => p e c H_exec c' H_trans.
+inversion H_exec as [e' H_init H_suff H_eq].
 apply exec_intros.
+- pose proof (list_same_head e c c') as H_head.
+  move => c0 H_some.
+  rewrite -H_head in H_some.
+  by apply H_init.
+- move => pref c0 c1.
+  case => [|c2 suffx] H_pref.
+  * rewrite list_rearrange in H_pref.
+    have H_re: pref ++ c0 :: c1 :: nil = (pref ++ c0 :: nil) ++ c1 :: nil.
+      by rewrite list_rearrange.
+    rewrite H_re {H_re} in H_pref.
+    apply app_inj_tail in H_pref.
+    move: H_pref => [H_pref H_cc'].
+    apply app_inj_tail in H_pref.
+    move: H_pref => [H_e H_c].
+    by rewrite -H_cc' -H_c.
+  * apply (H_suff pref c0 c1 (removelast (c2 :: suffx))).
+    have H_rl : removelast (e ++ c :: c' :: nil) = removelast (pref ++ c0 :: c1 :: c2 :: suffx).
+      by rewrite H_pref.
+    have H_neq : c :: c' :: nil <> nil by [].    
+    rewrite (removelast_app e H_neq) /= {H_neq} in H_rl.
+    have H_re: pref ++ c0 :: c1 :: c2 :: suffx = (pref ++ c0 :: c1 :: nil) ++ c2 :: suffx.
+      by rewrite app_ass -app_comm_cons.
+    rewrite H_re {H_re} in H_rl.
+    have H_nnil: c2 :: suffx <> nil by [].
+    rewrite (removelast_app (pref ++ c0 :: c1 :: nil) H_nnil) {H_nnil} in H_rl.
+    by rewrite H_rl app_ass -app_comm_cons.
+Qed.
+  
+Lemma exec_impl_trans_star : forall p `(execution_of p e), trans_star p e.
+Proof.
+move => p e H_exec.
+inversion H_exec as [e' H_init H_suff H_eq].
+clear H_exec.
+move: e H_init H_suff H_eq. 
+elim => [H_init H_suff H_eq|c]; first by apply tr_star_nil.
+case => [|c' l] H_init H_suff H_eq H; first by apply tr_star_sing.
+apply tr_star_step; first by apply H_eq with (pref := nil) (suff := l).
+apply H_init.
+Focus 2.
+- move => pref c0 c1 suffx H_eq_suffx.
+  apply H_eq with (pref := c :: pref) (suff := suffx).
+  by rewrite H_eq_suffx.
+Focus 2.
+- 
+F
 
-pose proof (list_same_head e c c').
-rewrite H2 in H.
-assumption.
 
-destruct suff.
-intros.
-rewrite list_rearrange in H2.
-assert (pref ++ c0 :: c'0 :: nil = (pref ++ c0 :: nil) ++ c'0 :: nil).
-  rewrite list_rearrange.
-  reflexivity.
-rewrite H3 in H2.
-apply app_inj_tail in H2.
-elim H2; clear H2; intros.
-apply app_inj_tail in H2.
-elim H2; clear H2; intros.
-subst.
-assumption.
-
-intros.
-apply (H0 pref c0 c'0 (removelast (c1 :: suff))).
-
-assert (forall (A: Set) (l l': list A), l = l' -> removelast l = removelast l').
-  intros; subst; reflexivity.
-
-apply H3 in H2.
-assert (H_tmp : c :: c' :: nil <> nil).
-  intro; discriminate.
-rewrite (removelast_app e H_tmp) in H2; clear H_tmp.
-simpl in H2.
-assert (pref ++ c0 :: c'0 :: c1 :: suff = (pref ++ c0 :: c'0 :: nil) ++ c1 :: suff).
-  rewrite app_ass.
+- move => c0 H_head.
+  apply (H_suff c0).
+  simpl.
+  simpl in H_head.
+  apply H0 with (pref := a :: pref) (suff := suff).
   rewrite <- app_comm_cons.
+  rewrite H.
   reflexivity.
-rewrite H4 in H2.
-assert (H_nnil : c1 :: suff <> nil).
-  intro; discriminate.
-rewrite (removelast_app (pref ++ c0 :: c'0 :: nil) H_nnil) in H2.
-rewrite H2.
-rewrite app_ass.
-rewrite <- app_comm_cons.
-rewrite list_rearrange3.
-assert (forall (A: Set) (l : list A), nil ++ l = l).
-  reflexivity.
-rewrite H5.
-reflexivity.
 Qed.
 
+Definition complete_execution_of p ex : Prop :=
+  execution_of p ex /\ ~exists c', execution_of p (ex ++ c' :: nil).
 
-  
-  Lemma exec_impl_trans_star : forall p `(execution_of p e), trans_star p e.
-  Proof.
-    intros.
-    inversion execution_of0; subst.
-    clear execution_of0 H.
-    induction e.
-    apply tr_star_nil.
-    induction e.
-    apply tr_star_sing.
-    apply tr_star_step.
-    apply H0 with (pref := nil) (suff := e).
-    reflexivity.
-    apply IHe.
-    intros.
-    apply H0 with (pref := a :: pref) (suff := suff).
-    rewrite <- app_comm_cons.
-    rewrite H.
-    reflexivity.
-  Qed.
-  
-  
-  Definition complete_execution_of p ex : Prop :=
-    execution_of p ex /\ ~exists c', execution_of p (ex ++ c' :: nil).
-  
-  
-  Inductive normal_conf : conf -> Prop :=
-  | is_norm_conf : forall h c m pc s ls ars gv, normal_conf (gv, h, (normal c m pc s ls)::ars).
-  
-  
-  Inductive exceptional_conf : conf -> Prop :=
-  | is_exc_conf : forall h o ars gv, exceptional_conf (gv, h, (exceptional o)::ars).
-  
-  
-  Inductive calling_conf p : conf -> Prop :=
-  | call_conf : forall gv h c m pc l ls ars,
-    trans p (gv, h, ars) (gv, h, (normal c m pc l ls)::ars) ->
-    calling_conf p (gv, h, ars).
-  
-  
-  Inductive returning_conf p : conf -> Prop :=
-  | ret_norm_conf : forall h ar ars,
-    trans p (h, ar::ars) (h, ars) ->
-    returning_conf p (h, ar::ars).
-  
-  
-  Definition visible_conf p c : Prop :=
-    calling_conf p c \/ returning_conf p c.
+Inductive normal_conf : conf -> Prop :=
+| is_norm_conf : forall h c m pc s ls ars gv, 
+    normal_conf (gv, h, (normal c m pc s ls)::ars).
 
-End program_model.
+Inductive exceptional_conf : conf -> Prop :=
+| is_exc_conf : forall h o ars gv, exceptional_conf (gv, h, (exceptional o)::ars).
+
+Inductive calling_conf p : conf -> Prop :=
+| call_conf : forall gv h c m pc l ls ars,
+  trans p (gv, h, ars) (gv, h, (normal c m pc l ls)::ars) ->
+  calling_conf p (gv, h, ars).
+
+Inductive returning_conf p : conf -> Prop :=
+| ret_norm_conf : forall h ar ars,
+  trans p (h, ar::ars) (h, ars) ->
+  returning_conf p (h, ar::ars).
+
+Definition visible_conf p c : Prop :=
+  calling_conf p c \/ returning_conf p c.
+
+End ProgramModel.
