coq/pcc/java_basic_defs.v
@@ -1,33 +1,31 @@
-
 Require Export ZArith.
 Require Export List.
 
-Section java_basic_defs.
+Section JavaBasicDefs.
   
-  Definition classid := nat.
-  Definition methid := nat.
-  Definition fieldid := nat.
-  Definition label := nat.
-  Definition loc := nat.
+Definition classid := nat.
+Definition methid := nat.
+Definition fieldid := nat.
+Definition label := nat.
+Definition loc := nat.
+
+Inductive jvalue :=
+| intval  (_: Z)
+| boolval (_: bool)
+| refval  (_: loc)
+| undefval.           (* used for, say 5 = true *)
+
+Inductive value :=
+| jval (_: jvalue)
+| ghost_errval.       (* represents \bot *)
+
+Coercion jval : jvalue >-> value.
+
+Definition object := fieldid -> jvalue.
+Definition stack := list jvalue.
+Definition emptystack : stack := nil.
   
-  
-  Inductive jvalue :=
-  | intval  (_: Z)
-  | boolval (_: bool)
-  | refval  (_: loc)
-  | undefval.           (* used for, say 5 = true *)
-  
-  Inductive value :=
-  | jval (_: jvalue)
-  | ghost_errval.       (* represents \bot *)
-  
-  Coercion jval : jvalue >-> value.
-  
-  Definition object := fieldid -> jvalue.
-  Definition stack := list jvalue.
-  Definition emptystack : stack := nil.
-  
-End java_basic_defs.
+End JavaBasicDefs.
 
 Notation "s '[[' n ']]'" := (nth n s undefval) (at level 90).
 
